rewrote proofs

proofs/trees.v
@@ -1,7 +1,71 @@
 From BalancedTrees Require Import definitions utils.
 
-Definition is_higher_rank (k1: A) (k2 : A) : bool :=
-  (rank_of k2 <? rank_of k1) || ((rank_of k1 =? rank_of k2) && (k1 <? k2)).
+Ltac get_couples :=
+  match goal with
+    | H: (_, _) = (_, _) |- _ => inversion H; subst end.
+
+Definition is_higher_rank (k1 : option A) (k2 : option A) : Prop :=
+  match k1, k2 with
+  | Some k1, Some k2 => (rank_of k2 < rank_of k1) \/ (rank_of k1 = rank_of k2 /\ k1 < k2)
+  | None, Some _ => True
+  | _, None => False
+  end.
+
+Notation "k1 '≻' k2" := (is_higher_rank k1 k2) (at level 70).
+Notation "k1 '!≻' k2" := (is_higher_rank (Some k1) (Some k2)) (at level 70).
+
+Definition is_higher_rankb (k1: option A) (k2 : option A) : bool :=
+  match k1, k2 with
+  | Some k1, Some k2 => (rank_of k2 <? rank_of k1) || ((rank_of k1 =? rank_of k2) && (k1 <? k2))
+  | None, Some _ => true
+  | _, None => false
+  end.
+
+Notation "k1 '≻?' k2" := (is_higher_rankb k1 k2) (at level 70).
+Notation "k1 '!≻?' k2" := (is_higher_rankb (Some k1) (Some k2)) (at level 70).
+
+Lemma is_higher_rank_dec : forall k1 k2, k1 ≻ k2 <-> k1 ≻? k2 = true.
+  intros k1 k2. destruct k1, k2; simpl; intuition try lia.
+  - apply Nat.ltb_lt in H0. rewrite H0. apply orb_true_l.
+  - apply Nat.ltb_lt in H1. apply Nat.eqb_eq in H. rewrite H, H1. simpl. apply orb_true_r.
+  - apply orb_prop in H. intuition.
+    + apply Nat.ltb_lt in H0. auto.
+    + apply andb_prop in H0. intuition. apply Nat.eqb_eq in H. apply Nat.ltb_lt in H1. auto.
+Qed.
+
+Lemma is_higher_rank_tricho : forall k k0,
+    is_higher_rank k k0 \/ k = k0 \/ is_higher_rank k0 k.
+  intros. destruct k, k0; unfold is_higher_rank; auto.
+  destruct (Nat.lt_trichotomy (rank_of a0) (rank_of a)) as [H | [H | H]]; auto.
+    destruct (Nat.lt_trichotomy a a0) as [H0 | [H0 | H0]]; auto.
+Qed.
+
+Definition is_higher_rank_than_rootb (k : option A) (t: Tree) : bool :=
+  match t with
+  | Leaf => true
+  | Node _ k1 _ => k ≻? (Some k1)
+  end.
+
+Definition is_higher_rank_than_root (k : option A) (t: Tree) : Prop :=
+  match t with
+  | Leaf => True
+  | Node _ k1 _ => k ≻ (Some k1)
+  end.
+
+Ltac get_root :=
+  match goal with
+    | H : is_higher_rank_than_root _ (Node _ _ _) |- _ => unfold is_higher_rank_than_root in H end.
+
+Lemma is_higher_rank_than_root_trans : forall t x x0,
+    is_higher_rank x0 x ->
+    is_higher_rank_than_root x t ->
+    is_higher_rank_than_root x0 t.
+  intros. destruct x, x0; destruct t; auto.
+  - simpl. inversion H; inversion H0; intuition eauto using Nat.lt_trans; lia.
+  - inversion H.
+Qed.
+
+Opaque is_higher_rank.
 
 (* coupe t en 2 sous-arbre : les éléments plus petits et les éléments plus grands *)
 Equations unzip (t: Tree) (k: A) : Tree * Tree :=
@@ -23,7 +87,7 @@ Equations unzip (t: Tree) (k: A) : Tree * Tree :=
 
 Equations insert (t: Tree) (k: A) : Tree :=
 | Leaf, k => singleton_list k
-| Node t1 kt t2, k with is_higher_rank kt k => {
+| Node t1 kt t2, k with kt !≻? k => {
   | false with unzip (Node t1 kt t2) k => {
       | (st, gt) => Node st k gt
     }
@@ -33,20 +97,14 @@ Equations insert (t: Tree) (k: A) : Tree :=
     }
   }.
 
-Definition is_higher_rank_than_root (t: Tree) (k: A) : bool :=
-  match t with
-  | Leaf => true
-  | Node _ k1 _ => is_higher_rank k k1
-  end.
-
-Inductive heap_higher_rank: Tree -> Prop :=
-| leaf_heap : heap_higher_rank Leaf
+Inductive heap: Tree -> Prop :=
+| leaf_heap : heap Leaf
 | rec_heap : forall t1 k t2,
-    heap_higher_rank t1 -> heap_higher_rank t2 ->
-    is_higher_rank_than_root t1 k = true -> is_higher_rank_than_root t2 k = true ->
-    heap_higher_rank (Node t1 k t2).
+    heap t1 -> heap t2 ->
+    is_higher_rank_than_root (Some k) t1 -> is_higher_rank_than_root (Some k) t2 ->
+    heap (Node t1 k t2).
 
-Definition zip_tree (t: Tree) : Prop := heap_higher_rank t /\ abr t.
+Definition zip_tree (t: Tree) : Prop := heap t /\ abr t.
 
 #[local] Hint Rewrite app_assoc: app.
 
@@ -55,12 +113,11 @@ Lemma unzip_elts_occurs_k : forall t k a b, abr t ->
     elements t = elements a ++ [k] ++ elements b.
 Proof.
   intros t k. funelim (unzip t k); try easy.
-  - intros. subst. apply Nat.eqb_eq in H. subst. rewrite <- Heqcall in *. inversion H1. subst. auto.
-  - intros. rewrite <- Heqcall in *. inversion H2. subst. simp elements. autorewrite with app. repeat f_equal.
-    rewrite <- app_assoc.
-    apply abr_node in H1 as Habr. intuition. apply Hind; auto. apply Nat.ltb_lt in H0.
+  - intros. subst. rewrite Nat.eqb_eq in *. subst. rewrite <- Heqcall in *. get_couples. auto.
+  - intros. rewrite <- Heqcall in *. get_couples. simp elements. autorewrite with app. repeat f_equal.
+    rewrite <- app_assoc. apply abr_node in H1 as Habr. intuition. apply Hind; auto. apply Nat.ltb_lt in H0.
     eapply abr_lt_occurs; eauto.
-  - intros. rewrite <- Heqcall in *. inversion H2. subst. simp elements.
+  - intros. rewrite <- Heqcall in *. get_couples. simp elements.
     replace ((elements t1 ++ [kt] ++ elements st2) ++ [k] ++ elements b)
       with (elements t1 ++ [kt] ++ elements st2 ++ [k] ++ elements b) by autorewrite with app using auto.
     repeat f_equal. apply abr_node in H1 as Habr. intuition. apply Hind; auto. apply opti_tricho in H; auto.
@@ -72,11 +129,13 @@ Lemma unzip_elts_not_occurs_k : forall t k a b,
 Proof.
   intros t k. funelim (unzip t k).
   - simp unzip. intros. inversion H0. auto.
-  - intros. rewrite Nat.eqb_eq in H. subst. absurd (kt ∈ Node t1 kt t2); auto.
-  - intros. rewrite <- Heqcall in *. inversion H2. subst. simp elements. autorewrite with app. repeat f_equal.
+  - intros. rewrite Nat.eqb_eq in *. subst. contradict H2. auto.
+  - intros. rewrite <- Heqcall in *. get_couples. simp elements. autorewrite with app. repeat f_equal.
     apply abr_node in H1 as Habr. intuition. apply Hind; eauto.
-  - intros. rewrite <- Heqcall in *. inversion H2. subst. simp elements. replace ((elements t1 ++ [kt] ++ elements st2) ++ elements b)
-      with (elements t1 ++ [kt] ++ elements st2 ++ elements b) by autorewrite with app using auto.
+  - intros. rewrite <- Heqcall in *. get_couples. simp elements.
+    replace ((elements t1 ++ [kt] ++ elements st2) ++ elements b)
+      with (elements t1 ++ [kt] ++ elements st2 ++ elements b)
+      by autorewrite with app using auto.
     repeat f_equal. apply abr_node in H1 as Habr. intuition. apply Hind; eauto.
 Qed.
 
@@ -85,7 +144,7 @@ Lemma unzip_elts_occursb : forall t k a b,
   intros t k. remember (occursb k t). destruct b.
   - apply eq_sym, occursb_correct in Heqb. intros. simpl delta. apply unzip_elts_occurs_k; auto.
   - apply eq_sym in Heqb. intros. simpl. eapply unzip_elts_not_occurs_k; eauto. intro.
-    apply occursb_correct in H1. rewrite Heqb in H1. discriminate.
+    apply occursb_correct in H1. congruence.
 Qed.
 
 Lemma unzip_preserves_abr_fst : forall t k a b,
@@ -107,10 +166,8 @@ Lemma unzip_smallers : forall t k a b, abr t -> unzip t k = (a, b) -> all_smalle
 Proof.
   intros t k. funelim (unzip t k).
   -  simp unzip. intros. inversion H0. subst. constructor.
-  - apply Nat.eqb_eq in H. subst. intros. apply abr_node in H. intuition. rewrite H0 in Heqcall.
-    inversion Heqcall. subst. auto.
-  - intros. apply abr_node in H1. specialize (Hind st1 gt1). intuition. rewrite H2 in Heqcall. inversion Heqcall.
-    subst. auto.
+  - apply Nat.eqb_eq in H. subst. intros. apply abr_node in H. intuition. congruence.
+  - intros. apply abr_node in H1. specialize (Hind st1 gt1). intuition. congruence.
   - intros. apply abr_node in H1. specialize (Hind st2 gt2). intuition. rewrite H2 in Heqcall. inversion Heqcall.
     subst. unfold all_smallers. simp elements. apply opti_tricho in H; auto.
     repeat (apply Forall_app; intuition eauto). eapply smaller_trans; eauto.
@@ -120,13 +177,11 @@ Lemma unzip_greaters : forall t k a b, abr t -> unzip t k = (a, b) -> all_greate
 Proof.
   intros t k. funelim (unzip t k).
   -  simp unzip. intros. inversion H0. subst. constructor.
-  - apply Nat.eqb_eq in H. subst. intros. apply abr_node in H. intuition. rewrite H0 in Heqcall.
-    inversion Heqcall. subst. auto.
+  - apply Nat.eqb_eq in H. subst. intros. apply abr_node in H. intuition. congruence.
   - intros. apply abr_node in H1. specialize (Hind st1 gt1). intuition. rewrite H2 in Heqcall. inversion Heqcall.
     subst. unfold all_greaters. simp elements. apply Nat.ltb_lt in H0.
     repeat (apply Forall_app; intuition eauto). eapply greater_trans; eauto.
-  - intros. apply abr_node in H1. specialize (Hind st2 gt2). intuition. rewrite H2 in Heqcall. inversion Heqcall.
-    subst. auto.
+  - intros. apply abr_node in H1. specialize (Hind st2 gt2). intuition. congruence.
 Qed.
 
 Lemma insert_elts : forall t k a b,
@@ -135,17 +190,18 @@ Proof.
   intros t k. funelim (insert t k).
   - simp unzip insert. intros. unfold singleton_list. inversion H0. auto.
   - rewrite <- Heqcall. intros. simp elements. remember (unzip t2 k). destruct p. specialize (H t t0).
-    apply abr_node in H0 as Habr. intuition. rewrite H. simp unzip in H1. rewrite Nat.eqb_sym in *. apply ltb_neqb in Heq as Hneq. apply ltb_antisymm in Heq.
-      rewrite Hneq, Heq in H1. simpl in H1. rewrite <- Heqp in H1. simpl in H1. inversion H1. subst. simp elements.
+    apply abr_node in H0 as Habr. intuition. rewrite H. simp unzip in H1. rewrite Nat.eqb_sym in *.
+    apply ltb_neqb in Heq as Hneq. apply ltb_antisymm in Heq.
+      rewrite Hneq, Heq in H1. simpl in H1. rewrite <- Heqp in H1. simpl in H1. get_couples. simp elements.
     repeat rewrite app_assoc. auto.
-  - rewrite <- Heqcall. intros. unfold is_higher_rank in *. assert (kt =? k = false).
+  - rewrite <- Heqcall. intros. unfold is_higher_rankb in *. assert (kt =? k = false).
     + apply Nat.eqb_neq. intro. subst. apply orb_prop in Heq0. intuition.
-      * rewrite Nat.ltb_irrefl in H2. discriminate.
-      * apply andb_prop in H2. intuition. rewrite Nat.ltb_irrefl in H4. discriminate.
+      * rewrite Nat.ltb_irrefl in *. discriminate.
+      * apply andb_prop in H2. intuition. rewrite Nat.ltb_irrefl in *. discriminate.
     + apply opti_tricho in Heq; auto. simp elements. remember (unzip t1 k). destruct p. specialize (H t t0).
       apply abr_node in H0 as Habr. intuition. rewrite H. simp unzip in H1. rewrite Nat.eqb_sym in H2.
-      rewrite H2 in H1. apply Nat.ltb_lt in Heq. rewrite Heq in H1. simpl in H1. rewrite <- Heqp in H1.
-      simpl in H1. inversion H1. simp elements. repeat (rewrite app_assoc). auto.
+      rewrite H2 in *. apply Nat.ltb_lt in Heq. rewrite Heq in H1. simpl in H1. rewrite <- Heqp in H1.
+      simpl in H1. get_couples. simp elements. autorewrite with app. auto.
   - rewrite <- Heqcall. rewrite Heq. simp elements. intros. inversion H0. subst. auto.
 Qed.
 
@@ -174,114 +230,95 @@ Proof. unfold abr.
   - constructor; auto. constructor.
   - eapply unzip_preserves_abr_snd; eauto.
   - apply pairwise_app_right_recipr.
-    assert (elements a ≺ [k])%stdpp by (eapply Forall_gt_direct, unzip_smallers; eauto). intuition auto.
-    eauto using pairwise_transitive_singleton.
-Qed.
-
-Lemma is_higher_rank_tricho : forall k k0,
-    is_higher_rank k k0 = true \/ k = k0 \/ is_higher_rank k0 k = true.
-  intros. unfold is_higher_rank. destruct (Nat.lt_trichotomy (rank_of k) (rank_of k0)) as [H | [H | H]].
-  - apply Nat.ltb_lt in H. rewrite H. auto.
-  - apply Nat.eqb_eq in H. rewrite H. rewrite Nat.eqb_sym in H. rewrite H.
-    destruct (Nat.lt_trichotomy k k0) as [H0 | [H0 | H0]]; auto;
-      apply Nat.ltb_lt in H0; rewrite H0; auto using orb_true_intro.
-  - apply Nat.ltb_lt in H. rewrite H. auto.
-Qed.
-
-Lemma is_higher_rank_than_root_trans : forall t x x0,
-    is_higher_rank x0 x = true ->
-    is_higher_rank_than_root t x = true ->
-    is_higher_rank_than_root t x0 = true.
-  intros. destruct t; auto. simpl. inversion H0. rewrite H2.
-  unfold is_higher_rank in *. apply orb_prop in H, H2. intuition (try apply andb_prop in H; try apply andb_prop in H2).
-  - apply orb_true_intro. left. rewrite Nat.ltb_lt in *. eauto using Nat.lt_trans.
-  - apply orb_true_intro. intuition. apply Nat.eqb_eq in H2. rewrite H2 in H1. auto.
-  - apply orb_true_intro. apply andb_prop in H1. intuition. apply Nat.eqb_eq in H2. rewrite H2 in *. auto.
-  - apply andb_prop in H1. intuition. rewrite Nat.ltb_lt, Nat.eqb_eq in *. rewrite H2, H1. apply orb_true_intro.
-    right. apply andb_true_intro. rewrite Nat.ltb_lt, Nat.eqb_eq. eauto using Nat.lt_trans.
+    assert (elements a ≺ [k])%stdpp by (eapply Forall_gt_direct, unzip_smallers; eauto).
+    intuition eauto using pairwise_transitive_singleton.
 Qed.
 
 Lemma unzip_preserves_is_higher_rank_than_root_fst : forall t k a b x,
     unzip t k = (a, b) ->
-    heap_higher_rank t ->
-    is_higher_rank_than_root t x = true ->
-    (*is_higher_rank x k ->*)
-    is_higher_rank_than_root a x = true.
+    heap t ->
+    is_higher_rank_than_root x t ->
+    is_higher_rank_than_root x a.
 Proof.
-  intros t k a b x. funelim (unzip t k).
-  - simp unzip. intros. inversion H. auto.
-  - intros. inversion H1. apply Nat.eqb_eq in H. rewrite H0 in Heqcall. inversion Heqcall. subst.
-    eauto using is_higher_rank_than_root_trans.
-  - rewrite <- Heqcall. intros. inversion H1. subst. specialize (Hind a gt1 x). inversion H2. subst. inversion H3.
-    rewrite H5. intuition. apply H6; eauto using is_higher_rank_than_root_trans.
-  - rewrite <- Heqcall. intros. inversion H1. intuition.
+  intros t k a b x. destruct x.
+  - funelim (unzip t k).
+    + simp unzip. intros. inversion H. auto.
+    + intros. inversion H1. apply Nat.eqb_eq in H. rewrite H0 in Heqcall. get_couples. get_root.
+      eauto using is_higher_rank_than_root_trans.
+    + rewrite <- Heqcall. intros. get_couples. specialize (Hind a gt1 a0). inversion H2. subst.
+      get_root. intuition eauto using is_higher_rank_than_root_trans.
+    + rewrite <- Heqcall. intros. inversion H1. intuition.
+  - intros. destruct a; constructor.
 Qed.
 
 Lemma unzip_preserves_is_higher_rank_than_root_snd : forall t k a b x,
     unzip t k = (a, b) ->
-    heap_higher_rank t ->
-    is_higher_rank_than_root t x = true ->
-    (*is_higher_rank x k ->*)
-    is_higher_rank_than_root b x = true.
+    heap t ->
+    is_higher_rank_than_root x t ->
+    is_higher_rank_than_root x b.
 Proof.
-  intros t k a b x. funelim (unzip t k).
-  - simp unzip. intros. inversion H. auto.
-  - intros. inversion H1. apply Nat.eqb_eq in H. rewrite H0 in Heqcall. inversion Heqcall. subst.
-    eauto using is_higher_rank_than_root_trans.
-  - rewrite <- Heqcall. intros. inversion H1. intuition.
-  - rewrite <- Heqcall. intros. inversion H1. subst. specialize (Hind st2 b x). inversion H2. subst. inversion H3.
-    rewrite H5. intuition. apply H6; eauto using is_higher_rank_than_root_trans.
+  intros t k a b x. destruct x.
+  - funelim (unzip t k).
+    + simp unzip. intros. inversion H. auto.
+    + intros. inversion H1. apply Nat.eqb_eq in H. rewrite H0 in Heqcall. get_couples. get_root.
+      eauto using is_higher_rank_than_root_trans.
+    + rewrite <- Heqcall. intros. get_couples. auto.
+    + rewrite <- Heqcall. intros. get_couples. specialize (Hind st2 b a0). inversion H2. subst.
+      get_root. intuition eauto using is_higher_rank_than_root_trans.
+  - intros. destruct b; constructor.
 Qed.
 
-Lemma unzip_preserves_heap_fst : forall t k a b, unzip t k = (a, b) -> heap_higher_rank t -> heap_higher_rank a.
+Lemma unzip_preserves_heap_fst : forall t k a b, unzip t k = (a, b) -> heap t -> heap a.
 Proof.
   intros t k a b. funelim (unzip t k).
-  - simp unzip. intros. inversion H. auto.
-  - rewrite <- Heqcall. intros. inversion H0. subst. inversion H1. auto.
-  - rewrite <- Heqcall. intros. inversion H1. subst. specialize (Hind a gt1). inversion H2. intuition auto.
-  - rewrite <- Heqcall. intros. inversion H1. subst. specialize (Hind st2 b). inversion H2.
+  - simp unzip. intros. get_couples. auto.
+  - rewrite <- Heqcall. intros. get_couples. inversion H1. auto.
+  - rewrite <- Heqcall. intros. get_couples. specialize (Hind a gt1). inversion H2. intuition auto.
+  - rewrite <- Heqcall. intros. get_couples. specialize (Hind st2 b). inversion H2.
     constructor; eauto using unzip_preserves_is_higher_rank_than_root_fst.
 Qed.
 
-Lemma unzip_preserves_heap_snd : forall t k a b, unzip t k = (a, b) -> heap_higher_rank t -> heap_higher_rank b.
+Lemma unzip_preserves_heap_snd : forall t k a b, unzip t k = (a, b) -> heap t -> heap b.
 Proof.
   intros t k a b. funelim (unzip t k).
   - simp unzip. intros. inversion H. auto.
-  - rewrite <- Heqcall. intros. inversion H0. subst. inversion H1. auto.
-  - rewrite <- Heqcall. intros. inversion H1. subst. specialize (Hind a gt1). inversion H2.
+  - rewrite <- Heqcall. intros. get_couples. inversion H1. auto.
+  - rewrite <- Heqcall. intros. get_couples. specialize (Hind a gt1). inversion H2.
     constructor; eauto using unzip_preserves_is_higher_rank_than_root_snd.
-  - rewrite <- Heqcall. intros. inversion H1. subst. specialize (Hind st2 b). inversion H2. intuition auto.
+  - rewrite <- Heqcall. intros. get_couples. specialize (Hind st2 b). inversion H2. intuition auto.
 Qed.
 
 Lemma insert_preserves_is_higher_rank_than_root : forall t k x,
-    is_higher_rank_than_root t x = true ->
-    is_higher_rank x k = true ->
-    is_higher_rank_than_root (insert t k) x = true.
-Proof. unfold is_higher_rank_than_root.
-  intros. destruct t.
-  - simp insert.
-  - inversion H. simp insert. remember (is_higher_rank a k). destruct b; simpl.
-    + destruct (a <? k); simpl; auto.
-    + destruct (unzip (Node t1 a t2) k). simpl. transitivity true; auto.
+    is_higher_rank_than_root x t ->
+    is_higher_rank x (Some k) ->
+    is_higher_rank_than_root x (insert t k).
+Proof.
+  unfold is_higher_rank_than_root. intros. destruct x.
+  - destruct t.
+    + simp insert. auto.
+    + simp insert. remember (a0 !≻? k). destruct b; simpl.
+      * apply eq_sym, is_higher_rank_dec in Heqb. destruct (a0 <? k); simpl; auto.
+      * destruct (unzip (Node t1 a0 t2) k). simpl. auto.
+  - destruct (insert t k); auto.
 Qed.
 
-Lemma insert_preserves_heap : forall t k, heap_higher_rank t -> heap_higher_rank (insert t k).
+Lemma insert_preserves_heap : forall t k, heap t -> heap (insert t k).
   intros t k. funelim (insert t k).
-  - simp insert. unfold singleton_list. auto using heap_higher_rank.
-  - intro. inversion H0. subst. intuition. rewrite <- Heqcall.
+  - simp insert. constructor; simpl; auto.
+  - intro. inversion H0. subst. intuition. rewrite <- Heqcall. apply is_higher_rank_dec in Heq0.
     constructor; auto using insert_preserves_is_higher_rank_than_root.
-  - intro. inversion H0. subst. intuition. rewrite <- Heqcall.
+  - intro. inversion H0. subst. intuition. rewrite <- Heqcall. apply is_higher_rank_dec in Heq0.
     constructor; auto using insert_preserves_is_higher_rank_than_root.
-  - intro H0.  inversion H0. subst. intuition. rewrite <- Heqcall.
+  - intro H0.  inversion H0. subst. intuition. rewrite <- Heqcall. 
     constructor; eauto using unzip_preserves_heap_fst, unzip_preserves_heap_snd.
-    + destruct (is_higher_rank_tricho kt k) as [Hrank | [Hrank | Hrank]].
-      * rewrite Heq0 in Hrank. discriminate.
-      * subst. simp unzip in Heq. rewrite Nat.eqb_refl in Heq. simpl in Heq. inversion Heq. subst. auto.
-      * eapply unzip_preserves_is_higher_rank_than_root_fst; eauto.
-    + destruct (is_higher_rank_tricho kt k) as [Hrank | [Hrank | Hrank]].
-      * rewrite Heq0 in Hrank. discriminate.
-      * subst. simp unzip in Heq. rewrite Nat.eqb_refl in Heq. simpl in Heq. inversion Heq. subst. auto.
-      * eapply unzip_preserves_is_higher_rank_than_root_snd; eauto.
+    + destruct (is_higher_rank_tricho (Some kt) (Some k)) as [Hrank | [Hrank | Hrank]].
+      * apply is_higher_rank_dec in Hrank. congruence.
+      * inversion Hrank. subst. simp unzip in Heq. rewrite Nat.eqb_refl in Heq. simpl in Heq. get_couples. auto.
+      * eauto using unzip_preserves_is_higher_rank_than_root_fst.
+    + destruct (is_higher_rank_tricho (Some kt) (Some k)) as [Hrank | [Hrank | Hrank]].
+      * apply is_higher_rank_dec in Hrank. congruence.
+      * inversion Hrank. subst. simp unzip in Heq. rewrite Nat.eqb_refl in Heq. simpl in Heq. get_couples. auto.
+      * eauto using unzip_preserves_is_higher_rank_than_root_snd.
 Qed.
 
 Theorem insert_correct : forall t k,
